experimental/ni_coq/vfiles/NIUtilTheorems.v
@@ -41,227 +41,218 @@ End misc.
 
 Section low_projection.
 
-Theorem flows_labeled_proj {A: Type}: forall ell (x: @labeled A),
-    (lbl x <<L ell) ->
-    (low_proj ell x) = x.
-Proof.
-    intros. destruct x. unfold low_proj. simpl in H.
-    destruct (lbl <<? ell); eauto; try contradiction.
-Qed.
-
-Theorem nflows_labeled_proj {A: Type}: forall ell (x: @labeled A),
-    ~(lbl x <<L ell) ->
-    (low_proj ell x) = Labeled A None (lbl x).
-Proof.
-    intros. destruct x. unfold low_proj. simpl in H.
-    destruct (lbl <<? ell); eauto; try contradiction.
-Qed.
-
-Definition idempotent {A: Type} (f: A -> A) := forall a, f (f a) = f a.
-
-Theorem labeled_low_proj_idempotent {A: Type}:
-    forall ell, idempotent (@low_proj A ell).
-Proof.
-    intros. unfold idempotent. intros x.
-    destruct x. unfold low_proj. destruct (lbl <<? ell)  eqn:Hflows;
-    rewrite Hflows; eauto.
-Qed.
-
-Definition node_low_proj_idempotent := @labeled_low_proj_idempotent node.
-Definition chan_low_proj_idempotent := @labeled_low_proj_idempotent channel.
-Definition event_low_proj_idempotent := @labeled_low_proj_idempotent event.
-
-Theorem state_low_proj_idempotent: forall ell, idempotent (state_low_proj ell).
-Proof.
-Admitted.
-
-Definition low_proj_loweq {A: Type}{a_low_proj: @low_proj_t A}
-    {a_low_eq: @low_eq_t A} := forall ell x,
-    (a_low_eq ell (a_low_proj ell x) x).
-
-Theorem labeled_low_proj_loweq {A: Type}:
-    @low_proj_loweq (@labeled A) low_proj low_eq.
-Proof.
-    unfold low_proj_loweq. unfold low_eq. unfold low_proj. intros.
-    destruct x. destruct (lbl <<? ell) eqn:Hflows;
-    rewrite Hflows; reflexivity.
-Qed.
-
-Definition node_low_proj_loweq := @labeled_low_proj_loweq node.
-Definition chan_low_proj_loweq := @labeled_low_proj_loweq channel.
-Definition event_low_proj_loweq := @labeled_low_proj_loweq event.
-
-Theorem state_low_proj_loweq: 
-    @low_proj_loweq state state_low_proj state_low_eq.
-Proof.
-Admitted.
-
-Theorem low_projection_preserves_lbl {A: Type}: forall ell (x: @labeled A),
-    (low_proj ell x).(lbl) = x.(lbl).
-Proof.
-    intros. destruct x. simpl. destruct (lbl <<? ell); auto.
-Qed.
-
-Definition node_projection_preserves_lbl :=
-    @low_projection_preserves_lbl node.
-Definition chan_projection_preserves_lbl := 
-    @low_projection_preserves_lbl channel.
-
-Theorem uncons_proj_chan_s: forall ell s han ch,
-    (chans (state_low_proj ell s)).[? han] = ch ->
-    exists ch',
-        (chans s).[? han] = ch' /\
-        low_proj ell ch' = ch.
-Proof.
-Admitted.
-
-Theorem uncons_proj_node_s': forall ell s id,
-    (nodes (state_low_proj ell s)).[? id] = 
-    (low_proj ell (nodes s).[? id]).
-Proof.
-    unfold state_low_proj. unfold fnd. unfold node_state_low_proj. simpl. intros.
-    destruct (lbl (nodes s id) <<? ell); try reflexivity.
-Qed.
-
-Theorem uncons_proj_node_s: forall ell s id n,
-    (nodes (state_low_proj ell s)).[? id] = n ->
-    exists n',
-        ((nodes s).[? id] = n') /\
-        (low_proj ell n') = n.
-Proof.
-    intros. rewrite uncons_proj_node_s' in H.
-    unfold fnd in *. unfold state_low_proj in *. simpl in *.
-    exists (nodes s id); split; eauto.
-Qed.
-
-Theorem state_nidx_to_proj_state_idx: forall ell s id n,
-    ((nodes s).[? id] = n) ->
-    ((nodes (state_low_proj ell s)).[? id] = (low_proj ell n)).
-Proof.
-Admitted.
-
-Theorem state_hidx_to_proj_state_hidx': forall ell s h,
-    (chans (state_low_proj ell s)).[? h] = (low_proj ell (chans s).[?h ]).
-Proof.
-Admitted.
-
-Theorem state_hidx_to_proj_state_hidx: forall ell s h ch,
-    ((chans s).[? h] = ch) ->
-    ((chans (state_low_proj ell s)).[? h] = (low_proj ell ch)).
-Proof.
-Admitted.
-
-(* TODO give better name *)
-Theorem proj_node_state_to_proj_n: forall ell s id nl n,
-    ((nodes (state_low_proj ell s)).[? id] = nl) ->
-    nl.(obj) = Some n ->
-    exists nl' n',
-        (nodes s).[? id] = nl' /\
-        (low_proj ell nl') = nl /\
-        nl'.(obj) = Some n'.
-Proof.
-Admitted.
-
-Theorem node_projection_preserves_flowsto: forall ell s id n n',
-    s.(nodes).[? id] = n ->
-    (state_low_proj ell s).(nodes).[? id] = n' ->
-    ~(n.(lbl) <<L ell) ->
-    ~(n'.(lbl) <<L ell).
-Proof.
-Admitted.
+  Theorem flows_labeled_proj {A: Type}: forall ell (x: @labeled A),
+      (lbl x <<L ell) ->
+      (low_proj ell x) = x.
+  Proof.
+      intros. destruct x. unfold low_proj. simpl in H.
+      destruct (lbl <<? ell); eauto; try contradiction.
+  Qed.
+  
+  Theorem nflows_labeled_proj {A: Type}: forall ell (x: @labeled A),
+      ~(lbl x <<L ell) ->
+      (low_proj ell x) = Labeled A None top.
+  Proof.
+      intros. destruct x. unfold low_proj. simpl in H.
+      destruct (lbl <<? ell); eauto; try contradiction.
+  Qed.
+  
+  Definition idempotent {A: Type} (f: A -> A) := forall a, f (f a) = f a.
+  
+  Theorem labeled_low_proj_idempotent {A: Type}:
+      forall ell, idempotent (@low_proj A ell).
+  Proof.
+      intros. unfold idempotent. intros x.
+      destruct x. unfold low_proj. destruct (lbl <<? ell)  eqn:Hflows.
+      rewrite Hflows; eauto. destruct (top <<? ell); reflexivity.
+  Qed.
+  
+  Definition node_low_proj_idempotent := @labeled_low_proj_idempotent node.
+  Definition chan_low_proj_idempotent := @labeled_low_proj_idempotent channel.
+  Definition event_low_proj_idempotent := @labeled_low_proj_idempotent event.
+  
+  Theorem state_low_proj_idempotent: forall ell, idempotent (state_low_proj ell).
+  Proof.
+  Admitted.
+  
+  Definition low_proj_loweq {A: Type}{a_low_proj: @low_proj_t A}
+      {a_low_eq: @low_eq_t A} := forall ell x,
+      (a_low_eq ell (a_low_proj ell x) x).
+  
+  Theorem labeled_low_proj_loweq {A: Type}:
+      @low_proj_loweq (@labeled A) low_proj low_eq.
+  Proof.
+      unfold low_proj_loweq. unfold low_eq. unfold low_proj. intros.
+      destruct x. destruct (lbl <<? ell) eqn:Hflows.
+      rewrite Hflows. reflexivity.
+      destruct (top <<? ell); reflexivity.
+  Qed.
+  
+  Definition node_low_proj_loweq := @labeled_low_proj_loweq node.
+  Definition chan_low_proj_loweq := @labeled_low_proj_loweq channel.
+  Definition event_low_proj_loweq := @labeled_low_proj_loweq event.
+  
+  Theorem state_low_proj_loweq: 
+      @low_proj_loweq state state_low_proj state_low_eq.
+  Proof.
+  Admitted.
+ 
+  (*
+  Theorem low_projection_preserves_lbl {A: Type}: forall ell (x: @labeled A),
+      (low_proj ell x).(lbl) = x.(lbl).
+  Proof.
+      intros. destruct x. simpl. destruct (lbl <<? ell); auto.
+  Qed.
+  
+  Definition node_projection_preserves_lbl :=
+      @low_projection_preserves_lbl node.
+  Definition chan_projection_preserves_lbl := 
+      @low_projection_preserves_lbl channel.
+  *)
+  
+  Theorem uncons_proj_chan_s: forall ell s han ch,
+      (chans (state_low_proj ell s)).[? han] = ch ->
+      exists ch',
+          (chans s).[? han] = ch' /\
+          low_proj ell ch' = ch.
+  Proof.
+  Admitted.
+  
+  Theorem uncons_proj_node_s': forall ell s id,
+      (nodes (state_low_proj ell s)).[? id] = 
+      (low_proj ell (nodes s).[? id]).
+  Proof.
+      unfold state_low_proj. unfold fnd. unfold node_state_low_proj. simpl. intros.
+      destruct (lbl (nodes s id) <<? ell); try reflexivity.
+  Qed.
+  
+  Theorem uncons_proj_node_s: forall ell s id n,
+      (nodes (state_low_proj ell s)).[? id] = n ->
+      exists n',
+          ((nodes s).[? id] = n') /\
+          (low_proj ell n') = n.
+  Proof.
+      intros. rewrite uncons_proj_node_s' in H.
+      unfold fnd in *. unfold state_low_proj in *. simpl in *.
+      exists (nodes s id); split; eauto.
+  Qed.
+  
+  Theorem state_nidx_to_proj_state_idx: forall ell s id n,
+      ((nodes s).[? id] = n) ->
+      ((nodes (state_low_proj ell s)).[? id] = (low_proj ell n)).
+  Proof.
+  Admitted.
+  
+  Theorem state_hidx_to_proj_state_hidx': forall ell s h,
+      (chans (state_low_proj ell s)).[? h] = (low_proj ell (chans s).[?h ]).
+  Proof.
+  Admitted.
+  
+  Theorem state_hidx_to_proj_state_hidx: forall ell s h ch,
+      ((chans s).[? h] = ch) ->
+      ((chans (state_low_proj ell s)).[? h] = (low_proj ell ch)).
+  Proof.
+  Admitted.
+  
+  (* TODO give better name *)
+  Theorem proj_node_state_to_proj_n: forall ell s id nl n,
+      ((nodes (state_low_proj ell s)).[? id] = nl) ->
+      nl.(obj) = Some n ->
+      exists nl' n',
+          (nodes s).[? id] = nl' /\
+          (low_proj ell nl') = nl /\
+          nl'.(obj) = Some n'.
+  Proof.
+  Admitted.
+  
+  Theorem node_projection_preserves_flowsto: forall ell s id n n',
+      s.(nodes).[? id] = n ->
+      (state_low_proj ell s).(nodes).[? id] = n' ->
+      ~(n.(lbl) <<L ell) ->
+      ~(n'.(lbl) <<L ell).
+  Proof.
+  Admitted.
 
 End low_projection.
 
 Section low_equivalence.
 
-
-Global Instance node_state_low_eq_refl: forall ell, Reflexive (node_state_low_eq ell) | 10.
-Proof. congruence. Qed.
-
-Global Instance node_state_low_eq_trans: forall ell, Transitive (node_state_low_eq ell) | 10.
-Proof. congruence. Qed.
-
-Global Instance node_state_low_eq_sym: forall ell, Symmetric (node_state_low_eq ell) | 10.
-Proof. congruence. Qed.
-
-Global Instance chan_state_low_eq_refl: forall ell, Reflexive (chan_state_low_eq ell) | 10.
-Proof. congruence. Qed.
-
-Global Instance chan_state_low_eq_trans: forall ell, Transitive (chan_state_low_eq ell) | 10.
-Proof. congruence. Qed.
-
-Global Instance chan_state_low_eq_sym: forall ell, Symmetric (chan_state_low_eq ell) | 10.
-Proof. congruence. Qed.
-
-Global Instance state_low_eq_refl: forall ell, Reflexive (state_low_eq ell) | 10.
-Proof. unfold state_low_eq. unfold Reflexive. eauto.  Qed.
-
-Global Instance state_low_eq_trans: forall ell, Transitive (state_low_eq ell) | 10.
-Proof. cbv [Transitive state_low_eq]. intros. destruct H, H0. split; congruence. Qed.
-
-Global Instance state_low_eq_sym: forall ell, Symmetric (state_low_eq ell) | 10.
-Proof. intros. unfold Symmetric. unfold state_low_eq. intros. destruct H. split; eauto.
-Qed.
-
-Global Instance event_low_eq_refl: forall ell, Reflexive (event_low_eq ell) | 10.
-Proof. congruence. Qed.
-
-Global Instance event_low_eq_trans: forall ell, Transitive (event_low_eq ell) | 10.
-Proof. congruence. Qed.
-
-Global Instance event_low_eq_sym: forall ell, Symmetric (event_low_eq ell) | 10.
-Proof. congruence. Qed.
-
-Theorem state_loweq_from_substates: forall ell s1 s2,
-    node_state_low_eq ell (nodes s1) (nodes s2) ->
-    chan_state_low_eq ell (chans s1) (chans s2) ->
-    state_low_eq ell s1 s2.
-Proof.
-  intros. unfold state_low_eq. unfold low_eq. unfold state_low_proj. eauto.
-Qed.
-
-Theorem state_loweq_to_deref_node: forall ell s1 s2 id n1,
-    (nodes s1).[? id] = n1 ->
-    (state_low_eq ell s1 s2) ->
-    exists n2,
-        (nodes s2).[? id] = n2 /\
-        (node_low_eq ell n1 n2).
-Proof.
-    intros. inversion H0. unfold node_state_low_proj in *. 
-Admitted. 
-
-Theorem node_low_eq_to_lbl_eq: forall ell n1 n2,
-    (node_low_eq ell n1 n2) ->
-    (n1.(lbl) = n2.(lbl)).
-Proof.
-    intros. inversion H.
-    assert ( lbl (low_proj ell n1) = lbl (low_proj ell n2)).
-    rewrite H1. reflexivity.
-    rewrite !node_projection_preserves_lbl in H0.
-    assumption.
-Qed.
-
-Theorem trace_leq_imples_head_st_leq: forall ell t1 t2 s1 s2,
-    (head_st t1 = Some s1) ->
-    (head_st t2 = Some s2) ->
-    (trace_low_eq ell t1 t2) ->
-    (state_low_eq ell s1 s2).
-Proof.
-    inversion 3. 
-    - 
-        exfalso. rewrite <- H3 in H. inversion H.
-    - 
-        assert (xs = s1). {
-            assert (head_st ((xs, xe) :: t0 ) = Some xs) by reflexivity.
-            congruence.
-        }
-
-        assert (ys = s2). {
-            assert (head_st ((ys, ye) :: t3 ) = Some ys) by reflexivity.
-            congruence.
-        }
-    congruence.
-Qed.
+  Global Instance node_state_low_eq_refl: forall ell, Reflexive (node_state_low_eq ell) | 10.
+  Proof. congruence. Qed.
+  
+  Global Instance node_state_low_eq_trans: forall ell, Transitive (node_state_low_eq ell) | 10.
+  Proof. congruence. Qed.
+  
+  Global Instance node_state_low_eq_sym: forall ell, Symmetric (node_state_low_eq ell) | 10.
+  Proof. congruence. Qed.
+  
+  Global Instance chan_state_low_eq_refl: forall ell, Reflexive (chan_state_low_eq ell) | 10.
+  Proof. congruence. Qed.
+  
+  Global Instance chan_state_low_eq_trans: forall ell, Transitive (chan_state_low_eq ell) | 10.
+  Proof. congruence. Qed.
+  
+  Global Instance chan_state_low_eq_sym: forall ell, Symmetric (chan_state_low_eq ell) | 10.
+  Proof. congruence. Qed.
+  
+  Global Instance state_low_eq_refl: forall ell, Reflexive (state_low_eq ell) | 10.
+  Proof. unfold state_low_eq. unfold Reflexive. eauto.  Qed.
+  
+  Global Instance state_low_eq_trans: forall ell, Transitive (state_low_eq ell) | 10.
+  Proof. cbv [Transitive state_low_eq]. intros. destruct H, H0. split; congruence. Qed.
+  
+  Global Instance state_low_eq_sym: forall ell, Symmetric (state_low_eq ell) | 10.
+  Proof. intros. unfold Symmetric. unfold state_low_eq. intros. destruct H. split; eauto.
+  Qed.
+  
+  Global Instance event_low_eq_refl: forall ell, Reflexive (event_low_eq ell) | 10.
+  Proof. congruence. Qed.
+  
+  Global Instance event_low_eq_trans: forall ell, Transitive (event_low_eq ell) | 10.
+  Proof. congruence. Qed.
+  
+  Global Instance event_low_eq_sym: forall ell, Symmetric (event_low_eq ell) | 10.
+  Proof. congruence. Qed.
+  
+  Theorem state_loweq_from_substates: forall ell s1 s2,
+      node_state_low_eq ell (nodes s1) (nodes s2) ->
+      chan_state_low_eq ell (chans s1) (chans s2) ->
+      state_low_eq ell s1 s2.
+  Proof.
+    intros. unfold state_low_eq. unfold low_eq. unfold state_low_proj. eauto.
+  Qed.
+  
+  Theorem state_loweq_to_deref_node: forall ell s1 s2 id n1,
+      (nodes s1).[? id] = n1 ->
+      (state_low_eq ell s1 s2) ->
+      exists n2,
+          (nodes s2).[? id] = n2 /\
+          (node_low_eq ell n1 n2).
+  Proof.
+      intros. inversion H0. unfold node_state_low_proj in *. 
+  Admitted. 
+  
+  Theorem trace_leq_imples_head_st_leq: forall ell t1 t2 s1 s2,
+      (head_st t1 = Some s1) ->
+      (head_st t2 = Some s2) ->
+      (trace_low_eq ell t1 t2) ->
+      (state_low_eq ell s1 s2).
+  Proof.
+      inversion 3. 
+      - 
+          exfalso. rewrite <- H3 in H. inversion H.
+      - 
+          assert (xs = s1). {
+              assert (head_st ((xs, xe) :: t0 ) = Some xs) by reflexivity.
+              congruence.
+          }
+  
+          assert (ys = s2). {
+              assert (head_st ((ys, ye) :: t3 ) = Some ys) by reflexivity.
+              congruence.
+          }
+      congruence.
+  Qed.
 
 End low_equivalence.
 
